\input{preamble}
\begin{document}
\author{Thomas Aarflot Storaas    $\qquad$    Erik Skaar  $\qquad$    Mikael Kiste}
\title{Report 2}
\maketitle


\textbf{We are a bit behind schedule. This is an incomplete report. For the newest version of the report visit \href{https://github.com/erikfsk/Project-2}{\textcolor{blue}{github}}.}

\section{Abstract}


\section{Introduction}
The aim of this project is to create a program that finds eigenvalues with Jacobi's(Givens') method. We start off with studying the quantum mechanical problem of a particle in an infinite potential well, generating a general solution to find the eigenvalues of a matrix. Then moving on to two particles with Coulomb interactions.

\section{Underlying theory}

For electrons it is safe to assume a sentro symmetric potential, making it reasonable to use spherical coordinates. Here the angle dependent parts of the Schr√∂dinger equation is independent of the position $r$. To model the electron further only the radial part of the SE is needed.

\begin{align}
	&-\frac{\hbar^2}{2m}\qty(\frac{1}{r^2}\pdv{r}r^2\pdv{r}-\frac{l(l+1)}{r^2})R(r)+V(r)R(r)=ER(r) &r\in[0,\infty)
\end{align}

Here $V(r)=(1/2)m\omega^2r^2$ the middle term can be expressed as $m\omega^2=k$. The eigenvalues($E$) are here the energy of the harmonic oscillator.  The frequency $\omega$ of the system are given as:

\begin{align}
	E_{nl}&=\hbar\omega\qty(2n+l+\frac{3}{2}) &n,l=0,1,2,3...
\end{align}

Here the variable $l$ is the orbital momentum of the electron. To further simplify the expression a substitution of variables can be made.
 
\begin{align*}
	-&\frac{\hbar^2}{2m}\qty(\frac{1}{r^2}\pdv{r}r^2\pdv{r}-\frac{l(l+1)}{r^2})R(r)+V(r)R(r)=ER(r)\\
	&R(r)=\frac{1}{r}u(r)\qquad \qquad u(0)=u(\infty)=0\\
	-&\frac{\hbar^2}{2m}\pdv[2]{u(r)}{r}+\qty(V(r)+\frac{l(l+1)}{r^2}\frac{hbar^2}{2m})u(r)=Eu(r)\\
\end{align*}

\subsection{Generalization}

To beam this specific example into a more general one dimensionless variables were introduced.
$\rho=(1/\alpha)r$ is introduced with $\alpha$ having the dimension length. $l$ is fixed to zero. 

\begin{align*}
	-\frac{\hbar^2}{2m\alpha^2}\pdv[2]{u(\rho)}{\rho}+V(\rho)u(\rho)=Eu(\rho)\\
\end{align*}

The potential is now defined to $V(\rho)=(1/2)k\alpha^2\rho^2$.

\begin{align*}
	-\frac{\hbar^2}{2m\alpha^2}\pdv[2]{u(\rho)}{\rho}+\frac{1}{2}k\alpha^2\rho^2u(\rho)=Eu(\rho)\\
	-\pdv[2]{u(\rho)}{\rho}+\frac{m}{\hbar^2}k\alpha^4\rho^2u(\rho)=\frac{2m\alpha^2}{\hbar^2}Eu(\rho)\\	
\end{align*}

To remove the units in the potential one can set $\alpha=\sqrt[4]{\frac{\hbar^2}{mk}}$, and the variables on the right hand side can be defined as $\lambda=\frac{2m\alpha^2}{\hbar^2}=E$
\begin{align}
	-\pdv[2]{u(\rho)}{\rho}+\rho^2u(\rho)=\lambda u(\rho)\label{general1particle}
\end{align}
This is now reduced to a general second derivative discrete function and can be expressed as:
\begin{align}
	\pdv[2]{u(\rho)}{\rho}=\frac{u(\rho+h)-2u(\rho)+u(\rho-h)}{h^2}+O(h^2)\label{generalwitherror}
\end{align}
Here $h$ is the step length. The limits of the new variable $\rho$ also needs to be defined. The lower limit, $r_{\mathrm{min}}=0\to\rho=0$ is fine, but the upper limit causes trouble. Here  $r_{\mathrm{max}}=\infty\to\rho=\infty$. This is not possible to represent on a computer. Since the function now has a discrete approximation a discrete value can also be given for the upper limit. $\rho=\rho_\mathrm{max}$. The step length will now be defined from the total amount of steps in the approximation.

\begin{align*}
	h=\frac{\rho_\mathrm{max}-\rho_\mathrm{min}}{N}
\end{align*} 

Indexing the steps after the number of steps taken will further be beneficial.
\begin{align*}
	\rho_0&\cdots\rho_i\cdots\rho_N \qquad \qquad i=0,1,2....N\\
	\rho_i&=\rho_0+hi
\end{align*}

Rewriting 
\begin{align}
	\pdv[2]{u(\rho)}{\rho}=\frac{u(\rho+h)-2u(\rho)+u(\rho-h)}{h^2}+O(h^2)
\end{align}

Applying the step-wise $\rho_i$ to the general result \ref{general1particle}, inserting \ref{generalwitherror} gives:

\begin{align*}
	-\frac{u(\rho_i+h)-2u(\rho_i)+u(\rho_i-h)}{h^2}+\rho_i^2u(\rho_i)=\lambda u(\rho_i)	
\end{align*}

A short hand notation of this would be to bring the variable the function $u$ works on into the subscript, $u(\rho_i)=u_i$.

\begin{align}
	-\frac{u_{i+1}-2u_i+u_{i-1}}{h^2}+V_i^2u_i=\lambda u_i
\end{align}

Systematizing this result into a matrix were a column represents $u_i$ will yield the following:

\begin{equation}
	\begin{bmatrix} \frac{2}{h^2}+V_1 & -\frac{1}{h^2} & 0   & 0    & \dots  &0     & 0 \\
		-\frac{1}{h^2} & \frac{2}{h^2}+V_2 & -\frac{1}{h^2} & 0    & \dots  &0     &0 \\
		0   & -\frac{1}{h^2} & \frac{2}{h^2}+V_3 & -\frac{1}{h^2}  &0       &\dots & 0\\
		\dots  & \dots & \dots & \dots  &\dots      &\dots & \dots\\
		0   & \dots & \dots & \dots  &-\frac{1}{h^2}  &\frac{2}{h^2}+V_{N-2} & -\frac{1}{h^2}\\
		0   & \dots & \dots & \dots  &\dots       &-\frac{1}{h^2} & \frac{2}{h^2}+V_{N-1}
	\end{bmatrix}
 	 \begin{bmatrix} u_{0} \\
		u_{1} \\
		\dots\\ \dots\\ \dots\\
		u_{N}
	\end{bmatrix}=\lambda\begin{bmatrix} u_{0} \\
	u_{1} \\
	\dots\\ \dots\\ \dots\\
	u_{N}
	\end{bmatrix}
	\label{eq:matrixse} 
\end{equation}
Note here that the end and start columns have been removed due to them being known from the boundary conditions. From the matrix one can define a better short hand notation for the values:

The diagonal matrix elements:
\begin{equation*}
d_i=\frac{2}{h^2}+V_i,
\end{equation*}
The non-diagonal matrix elements:
\begin{equation*}
e_i=-\frac{1}{h^2}.
\end{equation*}

\section{Method}

















\section{Result}
















\section{Discussion}
















\section{Conclusion}





















%\printbibliography

\end{document}